Relation translation of go.type -> load function works, but function
dispatch has to remain dynamic to avoid a false assumption when there's
mutual recursion.

new/golang/defn/mem.v
@@ -1,93 +1,7 @@
 From New.golang.defn Require Export typing intoval.
 From Perennial Require Import base.
 
-Module mem.
-Inductive type :=
-(* Boolean *)
-| boolT
-
-(* Numeric, except float and impl-specific sized objects *)
-| w8T
-| w16T
-| w32T
-| w64T
-| stringT
-| arrayT (n : nat) (elem : type)
-| sliceT
-| interfaceT
-| structT (decls : list (go_string * type))
-| ptrT
-| funcT
-| invalidT.
-
-Section val_types.
-  Context `{ffi_syntax}.
-
-  Fixpoint type_size (t : type) : nat :=
-    match t with
-    | structT d =>
-        (fix type_size_struct d : nat :=
-           match d with
-           | [] => O
-           | (_,t) :: d => (type_size t + type_size_struct d)%nat
-           end
-        ) d
-    | arrayT n e => n * (type_size e)
-    | _ => 1
-    end.
-End val_types.
-
-Reserved Notation "l +ₗ[ t ] z" (at level 50, left associativity, format "l  +ₗ[ t ]  z").
-Global Notation "l +ₗ[ t ] z" := (l +ₗ type_size t * z) : stdpp_scope .
-Global Notation "e1 +ₗ[ t ] e2" := (BinOp (OffsetOp (type_size t)) e1%E e2%E) : expr_scope .
-
-(** * Memory load, store, and allocation with type annotations. *)
-Section go_lang.
-  Context `{ffi_syntax}.
-  Context `{!NamedUnderlyingTypes}.
-
-  Fixpoint load (t : type) : val :=
-    match t with
-    | structT d =>
-        (fix load_struct d : val :=
-          match d with
-          | [] => (λ: <>, #())%V
-          | (_,t) :: d => (λ: "l", (load t "l", load_struct d ("l" +ₗ[t] #(W64 1))))%V
-          end) d
-    | arrayT n t =>
-        (fix load_array n : val :=
-          match n with
-          | O => (λ: <>, #())%V
-          | S n => (λ: "l", (load t "l", load_array n ("l" +ₗ[t] #(W64 1))))%V
-          end) n
-    | invalidT => (λ: "l", Panic "invalid type")%V
-    | _ => (λ: "l", !(Var "l"))%V
-    end.
-
-  Fixpoint store (t : type): val :=
-    match t with
-    | structT d =>
-        (fix store_struct d : val :=
-          match d with
-          | [] => (λ: <> <>, #())%V
-          | (f,t) :: d => (λ: "p" "v",
-                                  store t "p" (Fst "v");;
-                                  store_struct d (BinOp (OffsetOp (type_size t)) "p" #(W64 1))
-                                    (Snd "v"))%V
-          end) d
-    | arrayT n t =>
-        (fix store_array n : val :=
-          match n with
-          | O => (λ: <> <>, #())%V
-          | S n => (λ: "p" "v",
-                            store t "p" (Fst "v");;
-                            store_array n (BinOp (OffsetOp (type_size t)) "p" #(W64 1)) (Snd "v"))%V
-          end) n
-    | invalidT => (λ: "l", Panic "invalid type")%V
-    | _ => (λ: "p" "v", "p" <- "v")%V
-    end.
-End go_lang.
-End mem.
+Module go.
 
 (* built-in types *)
 Definition uint64 : go.type := go.Named "uint64"%go [].
@@ -98,64 +12,130 @@ Definition int64 : go.type := go.Named "int64"%go [].
 Definition int32 : go.type := go.Named "int32"%go [].
 Definition int16 : go.type := go.Named "int16"%go [].
 Definition int8 : go.type := go.Named "int8"%go [].
+Definition string : go.type := go.Named "string"%go [].
+Definition bool : go.type := go.Named "bool"%go [].
+Definition byte : go.type := uint8.
+Definition rune : go.type := uint32.
 
-Definition primitives : gmap go_string mem.type :=
-  {["uint64"%go := mem.w64T;
-    "uint32"%go := mem.w32T;
-    "uint16"%go := mem.w16T;
-    "uint8"%go := mem.w8T;
-    "int64"%go := mem.w64T;
-    "int32"%go := mem.w32T;
-    "int16"%go := mem.w16T;
-    "int8"%go := mem.w8T
-  ]}.
-
-Module go.
 Section defs.
 Context `{!NamedUnderlyingTypes}.
-
-Local Definition to_mem_type_aux (recur : go.type → mem.type) (t : go.type) : mem.type :=
-  match t with
-  | go.Named n [] =>
-      match primitives !! n with
-      | Some mt => mt
-      | None => recur (named_to_underlying n [])
-      end
-  | go.PointerType _ => mem.ptrT
-  | go.StructType field_decls =>
-      mem.structT
-        ((λ f, match f with
-               | go.FieldDecl fn ty => (fn, recur ty)
-               | go.EmbeddedField fn ty => (fn, recur ty)
-               end) <$> field_decls)
-  | _ => mem.invalidT
-  end.
-
-Local Definition to_mem_type_fuel (fuel : positive) : go.type → mem.type :=
-  Pos.peano_rect
-    (const (go.type → mem.type)) (λ _, mem.invalidT)
-    (λ _ recur, to_mem_type_aux recur)
-    fuel.
-
-Definition to_mem_type := to_mem_type_fuel 1024.
-
-Lemma to_mem_type_fuel_step fuel t :
-  (fuel ≠ 1)%positive →
-  to_mem_type_fuel fuel t =
-  (to_mem_type_aux (to_mem_type_fuel (fuel-1)) t).
-Proof.
-  intros Hf.
-  unfold to_mem_type_fuel.
-  replace (fuel) with (Pos.succ (fuel-1)) by lia.
-  rewrite Pos.peano_rect_succ.
-  f_equal. f_equal. lia.
-Qed.
-
 Context `{ffi_syntax}.
 
 Definition alloc_def (V : Type) `{!IntoVal V} : val := (λ: <>, ref #(zero_val V)).
 Program Definition alloc := sealed @alloc_def.
 Definition alloc_unseal : alloc = _ := seal_eq _.
+
+Inductive is_primitive : go.type → Prop :=
+| is_primitive_uint64 : is_primitive uint64
+| is_primitive_uint32 : is_primitive uint32
+| is_primitive_uint16 : is_primitive uint16
+| is_primitive_uint8 : is_primitive uint8
+| is_primitive_int64 : is_primitive int64
+| is_primitive_int32 : is_primitive int32
+| is_primitive_int16 : is_primitive int16
+| is_primitive_int8 : is_primitive int8
+| is_primitive_string : is_primitive string
+| is_primitive_bool : is_primitive bool
+
+| is_primitive_pointer t : is_primitive (go.PointerType t)
+| is_primitive_function sig : is_primitive (go.FunctionType sig)
+| is_primitive_interface elems : is_primitive (go.InterfaceType elems)
+| is_primitive_slice elem : is_primitive (go.SliceType elem)
+| is_primitive_map kt vt : is_primitive (go.MapType kt vt)
+| is_primitive_channel dir t : is_primitive (go.ChannelType dir t).
+
+Class MemOps :=
+{
+  load : go.type → val;
+  store : go.type → val;
+  size : go.type → Z;
+
+  is_load_underlying t : load t = load (to_underlying t);
+  is_load_primitive t (H : is_primitive t) : load t = (λ: "l", ! "l")%V;
+  is_load_struct fds :
+    let body := (foldl (λ '(offset, ld) (fd : go.field_decl),
+                          (offset,
+                             (ld, (match fd with
+                                   | go.FieldDecl _ t 
+                                   | go.EmbeddedField _ t => load t
+                                   end)
+                                    (BinOp (OffsetOp offset) #(W64 1) "l"))%E)
+                   ) (0, Val #()) fds) in
+    load (go.StructType fds) = (λ: "l", body.2)%V;
+  is_load_array n elem :
+    let body := (Z.iter n
+                   (λ '(offset, ld),
+                      (offset + 1,
+                         (ld, load elem
+                                (BinOp (OffsetOp (offset * size elem))
+                                   #(W64 1) "l"))%E)
+                   ) (0, Val #())) in
+    load (go.ArrayType n elem) = (λ: "l", body.2)%V;
+
+  size_underlying t : size t = size (to_underlying t);
+  size_primitive t (H : is_primitive t) : size t = 1;
+  size_struct fds : size (go.StructType fds) =
+                    foldl Z.add 0 ((λ fd, match fd with
+                                          | go.FieldDecl _ t
+                                          | go.EmbeddedField _ t => size t
+                                          end
+                                   ) <$> fds);
+  size_array n elem : size (go.ArrayType n elem) = n * size elem;
+}.
+
+Context `{!MemOps}.
+
+Record foo_t := 
+  mk {
+      a : w64;
+    }.
+Global Instance into_val_foo : IntoVal foo_t :=
+  {| to_val_def := λ v, (#v.(a), #())%V; zero_val := (mk (zero_val _)) |}.
+
+Definition foo : go.type := go.Named "foo"%go [].
+Definition foo_impl : go.type := go.StructType [(go.FieldDecl "a"%go uint64)].
+
+Class foo_type_assumptions : Prop :=
+  {
+    foo_underlying : named_to_underlying "foo"%go [] = foo_impl
+  }.
+
+Context `{!foo_type_assumptions}.
+
+Goal size (go.ArrayType 3 foo) = 3.
+  rewrite size_array size_underlying /= foo_underlying
+    size_struct /= size_primitive //. constructor.
+Qed.
+
+Definition struct_field_get (field_name : go_string) (t : go.type) : val :=
+  match to_underlying t with
+  | go.StructType fds =>
+      (* Look for the first field named `field_name`. *)
+      
+  end
+.
+
+Goal load (go.ArrayType 3 foo) = (λ: "l", ! "l")%V.
+  rewrite is_load_array /=. vm_compute Z.add.
+  rewrite is_load_underlying /=. foo_underlying.
+  rewrite is_load_struct /=.
+
+Goal load foo = (λ: "l", ! "l")%V.
+  rewrite is_load_underlying /= foo_underlying.
+  rewrite is_load_struct /=.
+
+  rewrite is_load_primitive; [|constructor].
+
+
+(* load t -> (load f1, load f2, load f3) when underlying(t) is a struct with
+   fields f1, f2, f3. *)
+Inductive is_load : go.type → val → Prop :=
+| is_load_uint64 t (H : is_primitive t) : is_load t (λ: "l", "l")%V
+| is_load_struct t fds (H : underlying t = go.StructType fds)
+                 (field_loads : list val)
+  :
+  is_load t (λ: "l", "l")%V
+.
 
 Definition load_def (t : go.type) : val := mem.load (to_mem_type t).
 Program Definition load := sealed @load_def.
